proof/correctness/avx2/MLKEM_InnerPKE_avx2_stack.ec
@@ -1,0 +1,34 @@
+require import AllCore IntDiv List.
+require import Jkem_avx2_stack MLKEM.
+from Jasmin require import JModel_x86.
+
+require import Array32 Array64 Array148 Array960 Array128 Array1088 Array1152 Array1184 Array2400.
+require import Array8 Array300 WArray64 WArray1184 WArray2400.
+import MLKEM InnerPKE.
+
+require import MLKEM_KEM_avx2.
+
+equiv mlkem_correct_kg_avx2_stack  : 
+M.__indcpa_keypair  ~ InnerPKE.InnerPKE.kg_derand :
+arg{1}.`3 = arg{2} ==> 
+    res{2}.`2 = Array1152.init ("_.[_]" res{1}.`2) /\
+    res{2}.`1.`1 = (init (fun (i : int) => res{1}.`1.[i]))%Array1152 /\
+    res{2}.`1.`2 = (init (fun (i : int) => res{1}.`1.[i + 1152]))%Array32.
+admitted.
+
+equiv mlkem_correct_enc_avx2_stack  : 
+M.__indcpa_enc  ~ InnerPKE.InnerPKE.enc_derand :
+arg{1}.`2 = arg{2}.`2 /\ arg{1}.`4 = arg{2}.`3 /\
+   Array1152.init(fun i => arg{1}.`3.[i]) = arg{2}.`1.`1 /\
+   Array32.init(fun i => arg{1}.`3.[i+1152]) = arg{2}.`1.`2 ==>
+   Array960.init(fun i => res{1}.[i]) = res{2}.`1 /\
+   Array128.init(fun i => res{1}.[i+960]) = res{2}.`2.
+admitted.
+
+equiv mlkem_correct_dec_avx2_stack  : 
+M.__indcpa_dec  ~ InnerPKE.InnerPKE.dec :
+arg{1}.`3 = arg{2}.`1 /\ 
+Array960.init(fun i => arg{1}.`2.[i]) = arg{2}.`2.`1 /\
+Array128.init(fun i => arg{1}.`2.[i+960]) = arg{2}.`2.`2  ==>
+   ={res}.
+admitted.
